\section{Z-transformation}
$$X(z)=\sum_{n=0}^{\infty}x(n)z^{-n}$$
Notation:
$$X(z)=\mathcal{Z}\{x(n)\}\qquad x(n)=\mathcal{Z}^{-1}\{X(z)\}$$
\subsubsection{s and z domain}

\subsection{Differential equations}
\subsection{Transfer Functions}
$$H(z)=\frac{Y(z)}{X(z)}$$
$H(z)$ is the transfer function.\\
$X(z)$ is the input sequence.\\
$Y(z)$ is the output sequence.

\subsection{Inverse Z-transformation}

\subsection{Examples}
\subsubsection{Example 1: Z-transformation}
\subsubsection{Example 2: Inverse Z-transformation}
