\section{Laplace transform}
Is a generalisation of the Fourier transform and defined as:
$$H(s)=\mathcal{L}\{h(t)\}=\int_{0^-}^{\infty}h(t)e^{ -st }  \, dt \quad\quad s \in\mathbb{C}$$
$s$ is a complex number $s=\sigma+j\omega$ and is identical with Fourier transform, if $s$ is set to $j\omega$.\\
Inverse Laplace tranformation:
$$h(t)=\mathcal{L}^{-1}\{H(t)\}=\frac{1}{2\pi j}\int_{\sigma_{c}-j\infty}^{\sigma_{c}+j\infty} H(s)e^{ st } \, ds $$
\begin{table}[h]
\centering
\begin{tabular}{|c|c|}
\hline
\cellcolor[HTML]{C0C0C0} \textbf{Signal}& \cellcolor[HTML]{C0C0C0}\textbf{Laplace Transform}  \\ \hline
1&$\frac{1}{s}$ \\ \hline
$e^{at}$& $\frac{1}{s-a}$ \\ \hline
$\sin(at)$&$\frac{a}{s^2+a^2}$ \\ \hline
$\cos(at)$&$\frac{s}{s^2+a^2}$ \\ \hline
\end{tabular}
\end{table}
\subsection{Examples}
\subsubsection{Example 1: Laplace Transform}
Using the Laplace transform, find the solution for the following equation:
$$\frac{\partial^{2}}{\partial t^{2}}y(t)+2\frac{\partial}{\partial t}y(t)+2y(t)=0$$
with initial conditions $y (0) = 1$ and $Dy (0) = -1$
\subsubsection{Example 2: Trabsfer Function}
Consider a mass-spring-damper system with the following differential equation:
$$m\overset{..}{x}=-kx-b\overset{.}{x}+f$$

Find the transfer function for the system with input $f$ and output $x$.

\rule{\textwidth}{0.5pt}

$$ms^2X(s)=-kX(s)-bsX(s)+F(s)$$
$$ms^2X(s)+kX(s)+bsX(s)=F(s)$$
$$(ms^2+k+bs)X(s)=F(s)$$
The transfer function is:
$$\frac{X(s)}{F(s)}=\displaystyle\frac{1}{ms^2+k+bs}$$
